#Simple start
## lvl 0 to 1 === State 1 to 2

E ( 2 ) = 1
E ( 1 ) = 1 + 0.5 * E ( 2 ) + 0.5 * E ( 1 )
  - 0.5 * E ( 1 ) = 0.5 * E ( 2 ) + 1
  - E ( 1 ) = E ( 2 ) + 2
  - E ( 1 ) =    1    + 2 
  - E ( 1 ) =    3


## lvl 0 to 2 === State 1 to 3
E ( 3 ) = 1 ---------------------------------------------Eq.1

E ( 1 ) = 1 + 0.5 * E ( 2 ) + 0.5 * E ( 1 )
  - 0.5 * E ( 1 ) = 0.5 * E ( 2 ) + 1
  - E ( 1 ) = E ( 2 ) + 2 -------------------------------Eq.2

E ( 2 ) = 1 + 0.5 * E ( 3 ) + 0.5 * E ( 1 )
  - combine Eq.2
  - E ( 2 ) = 1 + 0.5 * E ( 3 ) + 0.5 * ( E ( 2 ) + 2 )
  - E ( 2 ) = 1 + 0.5 * E ( 3 ) + 0.5 * E ( 2 ) + 1
  - 0.5 * E ( 2 ) = 1 + 0.5 * E ( 3 ) + 1
  - E ( 2 ) = E ( 3 ) + 4
  - combine Eq.1
  - E ( 2 ) =    1    + 4
  - E ( 2 ) =    5

E ( 1 ) =  E ( 2 ) + 2
  - E ( 1 ) =  5 + 2 = 7



